$$
\begin{gather}
\sum\limits_{i=1}^{n}iq^{i}={q\over 1-q}\left({1-q^{n}\over1-q}-nq^n\right)\\

\sum\limits_{i=m}^{n}i^{\underline{m}}x^{i-m}=m!{1\over(1-x)^{m+1}}-m!\sum\limits_{k=0}^{m}{(n+1)^{\underline{k}}\over k!}{x^{n+1-k}\over(1-x)^{m-k+1}}\\

\sum\limits_{k=1}^{n}(-1)^{k}k=(-1)^{n}\left\lfloor{n+1\over2}\right\rfloor\\

a_{n}=Aa_{n-1}+Ba_{n-2}\Rightarrow a_n=\begin{cases}\displaystyle
{a_{2}-\lambda a_{1}\over \mu-\lambda}\mu^{n-1}-{a_{2}-\mu a_{1}\over\mu-\lambda}\lambda^{n-1}&(\mu\neq \lambda)\\
\mu^{n-2}\left((n-1)a_{2}-(n-2)\mu a_{1}\right)&(\mu=\lambda)
\end{cases}

\end{gather}
$$
