**T20220910-8**

已知 $a_1,a_2,...,a_n>0$ 和 $0<b_1\le b_2\le...\le b_n$，又设
$$
a_1\le b_1\\
a_1+a_2\le b_1+b_2\\
a_1+a_2+a_3\le b_1+b_2+b_3\\
...\\
\sum_{i=1}^{n}a_i\le\sum_{i=1}^{n}b_i
$$
求证
$$
\prod_{i=1}^{n}a_i\le \prod_{i=1}^{n}b_i
$$
**证明**

注意到
$$
\left(\frac{1}{b_i}-\frac{1}{b_{i+1}}\right)\left(\sum_{j=1}^{i}a_j\right)\le \left(\frac{1}{b_i}-\frac{1}{b_{i+1}}\right)\left(\sum_{j=1}^{i}b_j\right)
$$
于是
$$
\sum_{i=1}^{n-1}\left(\frac{1}{b_i}-\frac{1}{b_{i+1}}\right)\left(\sum_{j=1}^{i}a_j\right)\le \sum_{i=1}^{n-1}\left(\frac{1}{b_i}-\frac{1}{b_{i+1}}\right)\left(\sum_{j=1}^{i}b_j\right)
$$
交换求和符号
$$
\sum_{j=1}^{n-1}a_j\sum_{i=j}^{n-1}\left(\frac{1}{b_i}-\frac{1}{b_{i+1}}\right)\le \sum_{j=1}^{n-1}b_j\sum_{i=j}^{n-1}\left(\frac{1}{b_i}-\frac{1}{b_{i+1}}\right)
$$
于是
$$
\sum_{j=1}^{n-1}a_j\left(\frac{1}{b_j}-\frac{1}{b_{n}}\right)\le \sum_{j=1}^{n-1}b_j\left(\frac{1}{b_j}-\frac{1}{b_{n}}\right)
$$
考虑到
$$
\frac{1}{b_n}\sum_{j=1}^{n}a_j\le\frac{1}{b_n}\sum_{j=1}^{n}b_j
$$
两式相加得
$$
\sum_{j=1}^{n}\frac{a_j}{b_j}\le n
$$
由均值不等式得
$$
n\sqrt[n]{\prod_{j=1}^{n}\frac{a_j}{b_j}}\le n
$$
于是原不等式成立。