**T20220910-9**

设 $n\in\mathbb{N}$，求证
$$
\sum_{k=1}^{n}\frac{1}{k}>n(\sqrt[n]{n+1}-1)
$$
**证明**

原不等式等价于
$$
\frac{1}{n}\sum_{k=1}^{n}\left(1+\frac{1}{k}\right)>\sqrt[n]{n+1}\\
\frac{1}{n}\sum_{k=1}^{n}\frac{k+1}{k}>\sqrt[n]{n+1}\\
$$
对不等式的左边运用均值不等式
$$
\frac{1}{n}\sum_{k=1}^{n}\frac{k+1}{k}>\sqrt[n]{\prod_{k=1}^{n}\frac{k+1}{k}}=\sqrt[n]{n+1}
$$
所以原不等式成立。

证毕。

这个例子的关键是利用
$$
\prod_{k=N}^{n}\frac{u_{k+1}}{u_k}=\frac{u_{n+1}}{u_N}
$$
这与
$$
\sum_{k=N}^{n}\frac{1}{k(k+1)}=\frac{1}{N}-\frac{1}{n+1}
$$
有异曲同工之妙。