$$
(a+b+c)^2=a^2+b^2+c^2+2ab+2bc+2ca
$$

[T20220910-3](../题库/T20220910-3.md) 解法二
$$
(a+b)(a+c)=bc+a(a+b+c)=a^2+(ab+bc+ca)
$$

[T20220910-4](../题库/T20220910-4.md) 解法二
$$
a^2+b^2+c^2\ge ab+bc+ca
$$

$$
(a+b+c)^2\ge3ab+3bc+3ca
$$

$$
(a+b)(b+c)(c+a)=2abc+ab(a+b)+bc(b+c)+ca(c+a)
$$

$$
8abc\le(a+b)(b+c)(c+a)
$$

$$
{z\over x+y}+{x\over y+z}+{y\over z+x}=-3+(x+y+z)\left({1\over x+y}+{1\over y+z}+{1\over z+x}\right)\ge{3\over2}
$$

$$
{a\over b}\ge 2\sqrt{4ab\cdot {a\over b}}-4ab=4(a-ab)
$$

$$
a_1\cdot{a_1-b_1\over a_1+b_1}+a_2\cdot{a_2-b_2\over a_2+b_2}\ge(a_1+a_2)\cdot{(a_1+a_2)-(b_1+b_2)\over (a_1+a_2)+(b_1+b_2)}
$$

当 $a_1b_2=a_2b_1$ 时取等。

$$
{a\over b}+{c\over d}\ge2\cdot{a+c\over b+d}\Leftrightarrow (ad-bc)(b-d)\le 0
$$

$$
(a+b+c)^3=\sum_{\text{cyc}}a^3+3\sum_{\text{cyc}}ab(b+c)+6abc
$$

$$
(a+b+c)(a^2+b^2+c^2)=\sum_{\text{cyc}}a^3+\sum_{\text{cyc}}ab(a+b)
$$

$$
\sum_{\text{cyc}}ab(a+b)=\sum_{\text{cyc}}a^2(b+c)=\sum_{\text{cyc}}a(b^2+c^2)
$$

$$
1+8x^3\le(1+2x^2)^2
$$

$$
(a+b+c)(a+b-c)(b+c-a)(c+a-b)=2\sum_{\text{cyc}}a^2b^2-\sum_{\text{cyc}}a^4
$$

当 $x\ge y\ge z>0$ 时有
$$
{x^2y\over z}+{y^2z\over x}+{z^2x\over y}\ge{x^2z\over y}+{y^2x\over z}+{z^2y\over x}
$$

$$
\frac{(2n)!!}{(2n+1)!!}>\frac{(2n-1)!!}{(2n)!!}
$$
注意，与上式相似的下式不成立
$$
\frac{(2n+1)!!}{(2n+2)!!}>\frac{(2n)!!}{(2n+1)!!}
$$
如 $n=1$ 时不成立。



当 $k\in\mathbb{N}^+$
$$
\sqrt{k+1}-\sqrt{k}<{1\over2\sqrt{k}}<\sqrt{k}-\sqrt{k-1}
$$



