$$
\begin{aligned}
&\text{ch}^2x-\text{sh}^2x=1\\
&\text{ch}(x+y)=\text{ch}x\text{ch}y+\text{sh}x\text{sh}y\\
&\text{sh}(x+y)=\text{sh}x\text{ch}y+\text{ch}x\text{sh}y\\
&\text{ch}x+\text{ch}y=2\text{ch}{x+y\over2}\text{ch}{x-y\over2}\\
&\text{ch}x-\text{ch}y=2\text{sh}{x+y\over2}\text{sh}{x-y\over2}\\
&\text{sh}x+\text{sh}y=2\text{sh}{x+y\over2}\text{ch}{x-y\over2}\\
&\text{ch}x\text{ch}y={1\over2}(\text{ch}(x+y)+\text{ch}(x-y))\\
&\text{sh}x\text{ch}y={1\over2}(\text{sh}(x+y)+\text{sh}(x-y))\\
&\text{sh}x\text{sh}y={1\over2}(\text{ch}(x+y)-\text{ch}(x-y)) \\
&\text{ash}(x)=\ln(x+\sqrt{x^2+1})\\
&\text{ach}(x)=\pm\ln(x-\sqrt{x^2-1})\\
\end{aligned}
$$

