**T20220717-7**

设数列 $\{x_n\}$ 与 $\{y_n\}$ 满足 $x_1=y_1=\sqrt{3}$，且
$$
x_{n+1}=x_n+\sqrt{1+x_n^2},\quad y_{n+1}={y_n\over1+\sqrt{1+y_n^2}}
$$
求证：当 $n>1$ 时，均有 $2<x_ny_n<3$

**证一**

注意到
$$
{1\over y_{n+1}}={1\over y_n}+\sqrt{1+{1\over y_n^2}}
$$
令 $\displaystyle z_n={1\over y_n}$，则 $\displaystyle z_1={1\over\sqrt{3}},\ z_2=\sqrt{3}=x_1$。

所以 $z_{n}=x_{n-1}$，故
$$
x_ny_n={x_n\over x_{n-1}}=1+\sqrt{1+{1\over x_{n-1}^2}}
$$
注意到 $\displaystyle 0\le{1\over x_{n-1}^2}\le{1\over3}$，所以原不等式成立。

**证二**

根据 $\displaystyle\cot{\alpha\over2}=\cot\alpha+\sqrt{1+\cot^2\alpha},\ \tan{\beta\over2}={\tan\beta\over1+\sqrt{1+\tan^2\beta}}$，令 $x_1=\cot \alpha,\ y_1=\tan\beta$，则 $\displaystyle x_{n}=\cot{\alpha\over2^{n-1}},\ y_{n}=\tan{\beta\over2^{n-1}}$。

因为 $\displaystyle \alpha={\pi\over 6},\ \beta={\pi\over3}$，故
$$
\begin{aligned}
x_ny_n&=\left(\cot{\beta\over2^{n-1}}+\sqrt{1+\cot^2{\beta\over2^{n-1}}}\right)\tan{\beta\over2^{n-1}}\\
&=1+\sqrt{1+\tan^2{\beta\over2^{n-1}}}
\end{aligned}
$$
注意到 $\displaystyle 0\le\tan^2{\beta\over2^{n-1}}\le\tan\beta={1\over3}$，所以原不等式成立。

上面两种证法本质上是等价的。



























