
记 $S_{n}=\sum\limits_{k=1}^{n}a_{k}$ 为 $\set{ a_{k}}$ 的部分和

### 计算 $S_{n}$ 的封闭形式

$$
\begin{gather}
\sum\limits_{k=0}^{n}x^{k}\\
\sum\limits_{k=m}^{n}k^{\underline{m}}x^{k-m}=m!{1\over(1-x)^{m+1}}-m!\sum\limits_{k=0}^{m}{(n+1)^{\underline{k}}\over k!}{x^{n+1-k}\over(1-x)^{m-k+1}}\\
\end{gather}
$$
### 幂级数

常见泰勒展开
$$
\begin{aligned}
e^{x}=&\sum\limits_{n=0}^{\infty}{x^{n}\over n!}\quad x\in(-\infty,+\infty)\\
\sin(x)=&\sum\limits_{n=0}^{\infty}{(-1)^{n}\over (2n+1)!}x^{2n+1}\quad x\in(-\infty,+\infty)\\
\cos(x)=&\sum\limits_{n=0}^{\infty}{(-1)^{n}\over (2n)!}x^{2n}\quad x\in(-\infty,+\infty)\\
\arctan(x)=&\sum\limits_{n=0}^{\infty}{(-1)^{n}\over 2n+1}x^{2n+1}\quad x\in[-1,+1]\\
\arcsin(x)=&x+\sum\limits_{n=1}^{\infty}{(2n-1)!\over (2n)!}{x^{2n+1}\over 2n+1}\quad x\in[-1,+1]\\
\sinh(x)=&\sum\limits_{n=0}^{\infty}{x^{2n+1}\over (2n+1)!}\quad x\in(-\infty,+\infty)\\
\rm{asinh}(x)=&\ln(x+\sqrt{x^{2}+1})\\
=&x+\sum\limits_{n=1}^{\infty}(-1)^{n}{(2n-1)!\over (2n)!}{x^{2n+1}\over 2n+1}\quad x\in(-\infty,+\infty)\\
\ln(1+x)=&\sum\limits_{n=1}^{\infty}{(-1)^{n+1}\over n}x^{n}\quad(x\in(-1,+1])\\
{1\over2}\ln \left({1+x\over 1-x}\right)=&\sum\limits_{n=0}^{\infty}{x^{2n+1}\over 2n+1}\quad x\in(-1,+1)
\end{aligned}
$$

### 傅里叶级数

以下收敛范围均为 $x\in [-\pi,\pi]$ 

$$
\begin{aligned}
|x|=&{\pi\over2}-{4\over\pi}\sum\limits_{n=1}^{\infty}{1\over (2n-1)^{2}}\cos nx\\
x^{2}=&{\pi^{2}\over 3}+\sum\limits_{n=1}^{\infty}{4(-1)^{n}\over n^{2}}\cos nx\\
|x^{3}|=&{\pi^{3}\over 4}+6\pi\sum\limits_{n=1}^{\infty}{(-1)^{n}\over n^{2}}\cos nx+{24\pi }\sum\limits_{n=1}^{\infty}{1\over(2n-1)^{4}}\cos nx\\
x^{4}=&{\pi^{4}\over 5}+8\pi^{2}\sum\limits_{n=1}^{\infty}{(-1)^{n}\over n^{2}}\cos nx+48\sum\limits_{n=1}^{\infty}{(-1)^{n+1}\over n^{4}}\cos nx\\
\cosh ax=&{e^{a\pi}-e^{-a\pi}\over 2a\pi}+{ae^{a\pi}-ae^{-a\pi}\over \pi}\sum\limits_{n=1}^{\infty}{(-1)^{n}\over a^{2}+n^{2}}\cos nx

\end{aligned}
$$
这些公式可用来计算
$$
\begin{aligned}
&\sum\limits_{n=1}^{\infty}{1\over n^{2}}={\pi^{2}\over 6}&\sum\limits_{n=1}^{\infty}{(-1)^{n+1}\over n^2}&={\pi^{2}\over 12}\\
&\sum\limits_{n=1}^{\infty}{1\over(2n-1)^{2}}={\pi^{2}\over 8}&\sum\limits_{n=1}^{\infty}{1\over(2n-1)^{4}}&={\pi^{4}\over 96}\\
&\sum\limits_{n=1}^{\infty}{1\over n^{4}}={\pi^{4}\over 90}&\sum\limits_{n=1}^{\infty}{(-1)^{n+1}\over n^{4}}&={\pi^{4}\over 720}\\
&\sum\limits_{n=1}^{\infty}{1\over a^{2}+n^{2}}={\pi\over 2a}\coth(a\pi)-{1\over 2a^{2}}&\sum\limits_{n=1}^{\infty}{(-1)^{n+1}\over a^{2}+n^{2}}&={1\over 2a^{2}}-{\pi\over 2a\sinh (a\pi)}\\
\end{aligned}
$$

对 $x^{2n}$ 求其在 $[-\pi,\pi]$ 上的傅里叶展开
$$
{a_{0}\over2}={\pi^{2n}\over 2n+1},\ a_{k}=(-1)^{k}\sum\limits_{i=1}^{n}{2(-1)^{i+1}(2n)^{\underline{2i-1}}\pi^{2n-2i}\over k^{2i}}
$$
记黎曼 $\displaystyle \zeta (x)=\sum\limits_{n=1}^{\infty}{1\over n^{x}}$，于是可得递推式
$$
\zeta(2n) =(-1)^{n+1}{n\pi^{2n}\over (2n+1)!}+\sum\limits_{i=1}^{n-1}(-1)^{n-i+1}{\pi^{2n-2i}\over(2n-2i+1)!}\zeta(2i)
$$
